src/common/Nemonuri.Bijective.IndexMap.fst
@@ -1,0 +1,18 @@
+module Nemonuri.Bijective.IndexMap
+
+module I = FStar.IntegerIntervals
+module ISet = Nemonuri.IndexSet
+module IMap = Nemonuri.IndexMap
+//open FStar.Bijection { ( =~ ) }
+//module B = FStar.Bijection
+module Seq = FStar.Seq.Base
+module List = FStar.List.Tot
+
+let bijective_index_map_predicate (#data_t:eqtype) (m:IMap.t data_t) =
+  m |> IMap.to_seq |> Seq.seq_to_list |> List.noRepeats
+
+type t (data_t:eqtype) = x:IMap.t data_t{bijective_index_map_predicate x}
+
+//let index_of 
+
+//let lemma_bijective_index_map 
