src/common/Nemonuri.Ensured.Premise.fst
@@ -1,0 +1,14 @@
+module Nemonuri.Ensured.Premise
+
+module En = Nemonuri.Ensured
+open FStar.Tactics.Typeclasses
+
+class t (data_t:Type) = {
+  fallback: data_t
+}
+
+let ensured_predicate #data_t {| premise:t data_t |} (data:data_t) = En.ensured_predicate premise.fallback data
+
+type ensured (data_t:Type) {| premise:t data_t |} = En.t premise.fallback
+
+
