src/common/Nemonuri.Ensured.fst
@@ -1,0 +1,8 @@
+module Nemonuri.Ensured
+
+
+let ensured_predicate (#data_t:Type) (fallback:data_t) (data:data_t) = fallback =!= data
+
+type t (#data_t:Type) (fallback:data_t) = x:data_t{ensured_predicate fallback x}
+
+//type from_premise (data_t:Type) {| p : premise data_t |} = 
