src/common/Nemonuri.Ref.fst
@@ -4,4 +4,14 @@ type t = {
   v: nat
 }
 
+let null = { v=0 }
 let is_null (ref:t) : Tot bool = ref.v = 0
+
+module Enp = Nemonuri.Ensured.Premise
+
+instance ensured_premise_t : Enp.t t =
+  {
+    fallback = null
+  }
+
+type ensured_t = Enp.ensured t
